michael_formal/drinks_machine.thy
@@ -158,17 +158,29 @@ lemma "observe_trace drinks (s0 drinks) <> [(''select'', [Str ''coke'']), (''coi
   apply (simp add: is_singleton_def the_elem_def possible_steps_q1 possible_steps_q2_coin possible_steps_q2_coin_2 possible_steps_q3_vend)
   by (simp add: transitions)
 
-lemma cat_impossible: "possible_steps drinks q2 <R (Suc 0) := Str ''coke'', R 2 := Num 0> ''cat'' [Num 50] = {}"
+lemma cat_impossible: "possible_steps drinks q2 d ''cat'' [Num 50] = {}"
   apply (simp add: possible_steps_def drinks_def)
   by (simp add: vend_def coin_def)
 
 (*Stop when we hit a spurious input*)
-lemma "observe_trace drinks (s0 drinks) <> [(''select'', [Str ''coke'']), (''cat'', [Num 50])] = [[]]"
+lemma select_cat: "observe_trace drinks (s0 drinks) <> [(''select'', [Str ''coke'']), (''cat'', [Num 50])] = [[]]"
   by (simp add: is_singleton_def the_elem_def possible_steps_q1 cat_impossible)
 
-lemma "\<not> (valid_trace (drinks) [(''select'', [Str ''coke'']), (''cat'', [Num 50])])"
-  apply (simp add: possible_steps_q1 cat_impossible)
-  by (simp add: transitions)
+lemma invalid_cat: "valid drinks q2 d' [(''cat'', [Num 50])] \<Longrightarrow> False"
+  apply (cases rule: valid.cases)
+    apply simp
+   apply simp
+  apply clarify
+  by (simp add: cat_impossible is_singleton_def)
+
+lemma "\<not> (valid_trace drinks [(''select'', [Str ''coke'']), (''cat'', [Num 50])])"
+  apply clarify
+  apply (cases rule: valid.cases)
+    apply simp
+   apply simp
+  apply clarify
+  apply (simp add: possible_steps_q1 invalid_cat)
+  using invalid_cat by force
 
 lemma "observe_trace drinks (s0 drinks) <> [(''select'', [Str ''coke'']), (''cat'', [Num 50]), (''coin'', [Num 50])] = [[]]"
   apply (simp add: possible_steps_q1 cat_impossible)
